\begin{sol}
    \begin{enumerate}
        \item \begin{proof}
            We have:
            \begin{align}
                & 1 =aa^{-1} \\
                \implies & (a^{-1})^{-1}(a^{-1}) = aa^{-1} \\ 
                \implies & (a^{-1})^{-1} = a
            \end{align}
            where the first implication is possible since $a^{-1} \in G$ and from the existence of the inverse. The second implication is possible due to right cancellation.
        \end{proof}
        \item \begin{proof}
            We propose that:
            \begin{equation}
                (a_1\cdots a_n)^{-1} = a_n^{-1}\cdots a_1^{-1}
            \end{equation}
            The base case $n=2$ was already proved in lecture, so we can skip to the inductive step. Suppose this is true for some $n=k$. Let us denote $a_1\cdots a_k = \alpha_k$. Then for $n=k+1$, we have:
            \begin{align}
                (a_1\cdots a_{k} a_{k+1})^{-1} &= (\alpha_k a_{k+1})^{-1} \\ 
                &= a_{k+1}^{-1} \alpha_k^{-1} & \text{(base case)} \\ 
                &= a_{k+1}^{-1}a_{k}^{-1}\cdots a_1^{-1} & \text{(inductive assumption)}
            \end{align}
            and we are done.
        \end{proof}
    \end{enumerate}
\end{sol}