\begin{sol}
    \begin{itemize}
        \item For $x^2=S$, we know that $x$ cannot be a rotation, since $x^2$ would also be a rotation. Therefore, let $x$ be the reflection:
        \begin{equation}
            x = sr^{a}
        \end{equation}
        Using the fact that $sr^{a} = r^{-a}s$, we have:
        \begin{align}
            x^2 &= (sr^{a})(sr^{a}) \\ 
            &= sr^{a}r^{-a}s \\ 
            &= s^2
        \end{align}
        Since $s$ is a reflection, then we must have $s^2=e$ and this is not possible.
        \item For $x^3=S$. we again cannot have a rotation. Let $x=sr^{a}$ and following the same steps as before:
        \begin{align}
            x^3 &= (sr^{a})(sr^{a})(sr^{a}) \\ 
            &= s^3r^{a} \\ 
            &= sr^{a} \\ 
            &= x
        \end{align}
        Therefore, this is satisfied iff $x=S$.
    \end{itemize}
\end{sol}